TestModels/resources/src/SimpleResourcesOperations.dfy
@@ -2,30 +2,24 @@
 // SPDX-License-Identifier: Apache-2.0
 
 include "../Model/SimpleResourcesTypes.dfy"
-include "./Config.dfy"
 include "./SimpleResource.dfy"
 
 module SimpleResourcesOperations refines AbstractSimpleResourcesOperations {
-  import Config
   import SimpleResource
 
-  // Polymorph's smithydafny demands InternalConfig
-  // exist in Operations
-  type InternalConfig = Config.Config
+  datatype Config = Config(
+    nameonly name: string
+  )
 
-  // Polymorph's smithydafny demands ValidInternalConfig? 
-  // exist in Operations
-  predicate ValidInternalConfig?(config: InternalConfig)
+  type InternalConfig = Config
+    
+  predicate method ValidInternalConfig?(config: InternalConfig)
   {
-    Config.ValidInternalConfig?(config)
+    && |config.name| > 0
   }
 
-  // Polymorph's smithydafny demands ModifiesInternalConfig
-  // exist in Operations
   function ModifiesInternalConfig(config: InternalConfig): set<object>
-  {
-    Config.ModifiesInternalConfig(config)
-  }
+  {{}}
   
   predicate GetResourcesEnsuresPublicly(
     input: GetResourcesInput,
@@ -40,19 +34,15 @@ module SimpleResourcesOperations refines AbstractSimpleResourcesOperations {
   )
     ensures output.Success? ==> output.value.output.ValidState()
   {
-    :- Need(Config.ValidInternalConfig?(config),
+    :- Need(ValidInternalConfig?(config),
       Types.SimpleResourceException(
       message := "Simple Resource Client has become invalid")
     );
-    :- Need(input.value.Some?,
-      Types.SimpleResourceException(
-      message := "Input Value MUST be set")
-    );
     var resource := new SimpleResource.SimpleResource(
-      input.value.value,
-      config
-     );
-     var result: GetResourcesOutput := GetResourcesOutput(
+      input.value,
+      config.name
+    );
+    var result: GetResourcesOutput := GetResourcesOutput(
       output := resource
     );
     return Success(result);  
